src/SemSeq.v
@@ -1,0 +1,38 @@
+Require Import Bool List String Peano_dec.
+Require Import Permutation.
+Require Import Common FMap Syntax Semantics.
+
+Inductive step_seq (sys: System) : State -> Label -> State -> Prop :=
+| SsSlt: forall s, step_seq sys s emptyLabel s
+| SsInt: forall oss oims obj idx mf os pos fmsg fpmsg fidx fchn outs,
+    In obj (sys_objs sys) ->
+    idx = obj_idx obj ->
+    oss@[idx] = Some os ->
+    oims@[idx] = Some mf ->
+
+    firstMF fidx fchn mf = Some fmsg ->
+    msg_id fmsg = pmsg_mid fpmsg ->
+    ValidMsgId fidx idx fchn fmsg ->
+    In fpmsg (obj_trs obj) ->
+    pmsg_precond fpmsg os ->
+    pmsg_postcond fpmsg os (msg_value fmsg) pos ->
+    outs = pmsg_outs fpmsg os (msg_value fmsg) ->
+
+    step_seq sys {| st_oss := oss; st_msgs := oims |}
+             (buildLabel nil (Some fmsg) (extOuts sys outs))
+             {| st_oss := oss +[ idx <- pos ];
+                st_msgs := distributeMsgs (intOuts sys outs) oims |}
+| SsExt: forall from emsgs oss oims,
+    ~ In from (indicesOf sys) ->
+    emsgs <> nil ->
+    SubList (map (fun m => msgTo (msg_id m)) emsgs) (indicesOf sys) ->
+    (* The only difference is here: a system accepts external messages only if
+     * it has no internal messages.
+     *)
+    EmptyM oims ->
+    step_seq sys {| st_oss := oss; st_msgs := oims |}
+             (buildLabel emsgs None nil)
+             {| st_oss := oss; st_msgs := distributeMsgs emsgs oims |}.
+
+Definition steps_seq := steps step_seq.
+
