src/SerialFacts.v
@@ -1,0 +1,12 @@
+Require Import Bool List String Peano_dec.
+Require Import Permutation.
+Require Import Common FMap Syntax Semantics SemDet SemSeq Serial.
+
+Theorem sequential_step_seq:
+  forall sys tr,
+    Behavior step_det sys tr ->
+    Sequential (historyOf sys tr) ->
+    Behavior step_seq sys tr.
+Proof.
+Admitted.
+
